add explicit return types for programs
almost works except that i cannot prove corr_sound anymore!
invoking "inversion" on the "exec" term produces an equality
of existT's like this:

H5 : existT (fun x : Set => result x) R (Halted v0) =
     existT (fun x : Set => result x) R r

which is similar to the problem described here

  http://stackoverflow.com/questions/24720137/inversion-produces-unexpected-existt-in-coq/24723398

except that we can't use inj_pair2_eq_dec (it seems unlikely
that Set is decidable).  does this mean we must restrict return
types to a fixed set of types?

src/HoareLogicN.v
@@ -8,18 +8,18 @@ Set Implicit Arguments.
 Definition addr := nat.
 Definition valu := nat.
 
-Inductive prog :=
-| Halt_ (v : valu)
-| Crash_
-| Read (a : addr)
-| Write (a : addr) (v : valu)
-| Seq (p1 : prog) (p2 : valu -> prog).
+Inductive prog : Set -> Type :=
+| Halt_ {R : Set} (v : R) : prog R
+| Crash_ (R : Set) : prog R
+| Read (a : addr) : prog valu
+| Write (a : addr) (v : valu) : prog unit
+| Seq {T R : Set} (p1 : prog T) (p2 : T -> prog R) : prog R.
 
 Notation "'Halt'" := Halt_.
 Notation "'Crash'" := Crash_.
 Notation "!" := Read.
 Infix "<--" := Write (at level 8).
-Notation "p1 ;; p2" := (Seq p1 (fun _ => p2)) (at level 9, right associativity).
+Notation "p1 ;; p2" := (Seq p1 (fun _: unit => p2)) (at level 9, right associativity).
 Notation "x <- p1 ; p2" := (Seq p1 (fun x => p2)) (at level 9, right associativity).
 
 Definition mem := addr -> valu.
@@ -27,18 +27,20 @@ Definition mem0 : mem := fun _ => 0.
 Definition upd (m : mem) (a : addr) (v : valu) : mem :=
   fun a' => if eq_nat_dec a' a then v else m a'.
 
-Inductive result :=
-| Halted (v : valu)
+Inductive result (R:Set) :=
+| Halted (v : R)
 | Crashed.
+Implicit Arguments Halted [R].
+Implicit Arguments Crashed [R].
 
-Inductive exec : mem -> prog -> mem -> result -> Prop :=
-| XHalt : forall m v, exec m (Halt v) m (Halted v)
+Inductive exec : forall {R : Set}, mem -> prog R -> mem -> result R -> Prop :=
+| XHalt : forall (R : Set) m (v : R), exec m (Halt v) m (Halted v)
 | XRead : forall m a, exec m (Read a) m (Halted (m a))
-| XWrite : forall m a v, exec m (Write a v) (upd m a v) (Halted 0)
-| XCrash : forall m p, exec m p m Crashed
-| XSeqC : forall m p1 p2 m', exec m p1 m' Crashed
-  -> exec m (Seq p1 p2) m' Crashed
-| XSeqH : forall m p1 p2 m' v m'' r, exec m p1 m' (Halted v)
+| XWrite : forall m a v, exec m (Write a v) (upd m a v) (Halted tt)
+| XCrash : forall (R : Set) m p, exec m p m (@Crashed R)
+| XSeqC : forall (R T : Set) m p1 p2 m', exec m p1 m' (@Crashed T)
+  -> exec m (Seq p1 p2) m' (@Crashed R)
+| XSeqH : forall (R T : Set) m p1 p2 m' (v : T) m'' (r : result R), exec m p1 m' (Halted v)
   -> exec m' (p2 v) m'' r
   -> exec m (Seq p1 p2) m'' r.
 
@@ -90,24 +92,24 @@ Definition diskIs (m : mem) : pred := eq m.
 
 (** ** Hoare triples *)
 
-Inductive corr :
-     pred             (* Precondition *)
-  -> prog             (* Program being verified *)
-  -> (result -> pred) (* Postcondition *)
+Inductive corr : forall {R : Set},
+     pred                (* Precondition *)
+  -> prog R              (* Program being verified *)
+  -> (@result R -> pred) (* Postcondition *)
   -> Prop :=
-| CHalt : forall pre v,
+| CHalt : forall (R:Set) pre (v:R),
   corr pre (Halt v) (fun r => [r = Crashed \/ r = Halted v] /\ pre)%pred
-| CCrash : forall pre,
-  corr pre Crash (fun r => [r = Crashed] /\ pre)%pred
+| CCrash : forall (R:Set) pre,
+  corr pre (Crash R) (fun r => [r = Crashed] /\ pre)%pred
 | CRead : forall pre a,
   corr pre (Read a) (fun r => exists v, a |-> v /\ [r = Crashed \/ r = Halted v] /\ pre)%pred
 | CWrite : forall pre a v,
-  corr pre (Write a v) (fun r => ([r = Crashed] /\ pre) \/ ([r = Halted 0] /\ pre[a <--- v]))%pred
-| CSeq : forall pre p1 p2 post1 post2,
+  corr pre (Write a v) (fun r => ([r = Crashed] /\ pre) \/ ([r = Halted tt] /\ pre[a <--- v]))%pred
+| CSeq : forall (R T:Set) pre p1 p2 post1 post2,
   corr pre p1 post1
-  -> (forall v, corr (post1 (Halted v)) (p2 v) post2)
-  -> corr pre (Seq p1 p2) (fun r => ([r = Crashed] /\ post1 Crashed) \/ post2 r)%pred
-| Conseq : forall pre post p pre' post', corr pre p post
+  -> (forall (v:T), corr (post1 (Halted v)) (p2 v) post2)
+  -> corr pre (Seq p1 p2) (fun r => ([r = @Crashed R] /\ post1 Crashed) \/ post2 r)%pred
+| Conseq : forall (R:Set) pre post p pre' post', @corr R pre p post
   -> (pre' --> pre)
   -> (forall r, post r --> post' r)
   -> corr pre' p post'.
@@ -129,7 +131,7 @@ Ltac pred := pred_unfold;
     intuition (try (congruence || omega);
       try autorewrite with core in *; eauto)).
 
-Lemma could_always_crash : forall pre p post, corr pre p post
+Lemma could_always_crash : forall R pre p post, @corr R pre p post
   -> forall m, pre m -> post Crashed m.
 Proof.
   induction 1; pred.
@@ -137,16 +139,19 @@ Qed.
 
 Local Hint Extern 1 =>
   match goal with
-    | [ |- _ Crashed _ ] =>
+    | [ |- _ (Crashed _) _ ] =>
       eapply could_always_crash; eassumption
   end.
 
-Theorem corr_sound : forall pre p post, corr pre p post
+Theorem corr_sound : forall R pre p post, @corr R pre p post
   -> forall m m' r, exec m p m' r
     -> pre m
     -> post r m'.
 Proof.
+  admit.
+(*
   induction 1; solve [ pred | inversion_clear 1; pred ].
+*)
 Qed.
 
 
@@ -159,21 +164,21 @@ Qed.
 
 Hint Resolve pimpl_refl.
 
-Fixpoint For_ (f : nat -> prog) (i n : nat) : prog :=
+Fixpoint For_ (f : nat -> prog unit) (i n : nat) : prog unit :=
   match n with
-    | O => Halt 0
+    | O => Halt tt
     | S n' => (f i);; (For_ f (S i) n')
   end.
 
-Theorem CFor : forall (f : nat -> prog)
+Theorem CFor : forall (f : nat -> prog unit)
   (nocrash : nat -> pred) (crashed : pred),
   (forall m, nocrash m --> crashed)
   -> forall n i,
     (forall m, i <= m < n + i
       -> {{nocrash m}} (f m)
-      {{r, ([r = Halted 0] /\ nocrash (S m)) \/ ([r = Crashed] /\ crashed)}})
+      {{r, ([r = Halted tt] /\ nocrash (S m)) \/ ([r = Crashed] /\ crashed)}})
     -> {{nocrash i}} (For_ f i n)
-    {{r, ([r = Halted 0] /\ nocrash (n + i)) \/ ([r = Crashed] /\ crashed)}}.
+    {{r, ([r = Halted tt] /\ nocrash (n + i)) \/ ([r = Crashed] /\ crashed)}}.
 Proof.
   induction n; simpl; intros.
 
@@ -210,69 +215,70 @@ Section prog'.
   (* This is a type that we pretend was passed as an extra
    * function argument, for specification purposes. *)
 
-  Inductive prog' :=
-  | Halt' (v : valu)
-  | Crash'
-  | Read' (a : addr)
-  | Write' (a : addr) (v : valu)
-  | Seq' (p1 : prog') (p2 : valu -> prog')
-  | If' P Q (b : {P} + {Q}) (p1 p2 : prog')
+  Inductive prog' : Set -> Type :=
+  | Halt' (R : Set) (v : R) : prog' R
+  | Crash' (R : Set) : prog' R
+  | Read' (a : addr) : prog' valu
+  | Write' (a : addr) (v : valu) : prog' unit
+  | Seq' {T R : Set} (p1 : prog' T) (p2 : T -> prog' R) : prog' R
+  | If' (R : Set) P Q (b : {P} + {Q}) (p1 p2 : prog' R) : prog' R
   | For' (nocrash : ghostT -> nat -> pred) (crashed : ghostT -> pred)
-    (f : nat -> prog') (n : nat)
-  | Call' (pre: ghostT -> pred) (p: prog) (post: ghostT -> result -> pred)
-    (c: forall g: ghostT, corr (pre g) p (post g)).
+    (f : nat -> prog' unit) (n : nat) : prog' unit
+  | Call' (R : Set) (pre: ghostT -> pred) (p: prog R)
+    (post: ghostT -> result R -> pred)
+    (c: forall g: ghostT, corr (pre g) p (post g)) : prog' R.
 
-  Fixpoint prog'Out (p : prog') : prog :=
+  Fixpoint prog'Out {R : Set} (p : prog' R) : prog R :=
     match p with
-      | Halt' v => Halt v
-      | Crash' => Crash
+      | Halt' _ v => Halt v
+      | Crash' R => Crash R
       | Read' a => Read a
       | Write' a v => Write a v
-      | Seq' p1 p2 => Seq (prog'Out p1) (fun x => prog'Out (p2 x))
-      | If' _ _ b p1 p2 => if b then prog'Out p1 else prog'Out p2
+      | Seq' _ _ p1 p2 => Seq (prog'Out p1) (fun x => prog'Out (p2 x))
+      | If' _ _ _ b p1 p2 => if b then prog'Out p1 else prog'Out p2
       | For' _ _ f n => For_ (fun x => prog'Out (f x)) 0 n
-      | Call' _ p _ _ => p
+      | Call' _ _ p _ _ => p
     end.
 
   Variable ghost : ghostT.
 
   (* Strongest postcondition *)
-  Fixpoint spost (pre : pred) (p : prog') : result -> pred :=
+  Fixpoint spost {R : Set} (pre : pred) (p : prog' R) : result R -> pred :=
     match p with
-      | Halt' v => fun r => [r = Crashed \/ r = Halted v] /\ pre
-      | Crash' => fun r => [r = Crashed] /\ pre
+      | Halt' _ v => fun r => [r = Crashed \/ r = Halted v] /\ pre
+      | Crash' _ => fun r => [r = Crashed] /\ pre
       | Read' a => fun r => exists v, a |-> v /\ [r = Crashed \/ r = Halted v] /\ pre
-      | Write' a v => fun r => ([r = Crashed] /\ pre) \/ ([r = Halted 0] /\ pre[a <--- v])
-      | Seq' p1 p2 => fun r => ([r = Crashed] /\ spost pre p1 Crashed)
+      | Write' a v => fun r => ([r = Crashed] /\ pre) \/ ([r = Halted tt] /\ pre[a <--- v])
+      | Seq' _ _ p1 p2 => fun r => ([r = Crashed] /\ spost pre p1 Crashed)
         \/ exists v, spost (spost pre p1 (Halted v)) (p2 v) r
-      | If' P Q b p1 p2 => fun r => spost (pre /\ [P]) p1 r
+      | If' _ P Q b p1 p2 => fun r => spost (pre /\ [P]) p1 r
         \/ spost (pre /\ [Q]) p2 r
       | For' nocrash crashed f n => fun r =>
-        ([r = Halted 0] /\ nocrash ghost n) \/ ([r = Crashed] /\ crashed ghost)
-      | Call' cpre cp cpost c => cpost ghost
+        ([r = Halted tt] /\ nocrash ghost n) \/ ([r = Crashed] /\ crashed ghost)
+      | Call' _ cpre cp cpost c => cpost ghost
     end%pred.
 
   (* Verification conditions *)
-  Fixpoint vc (pre : pred) (p : prog') : Prop :=
+  Fixpoint vc {R : Set} (pre : pred) (p : prog' R) : Prop :=
     match p with
-      | Halt' v => True
-      | Crash' => True
+      | Halt' _ v => True
+      | Crash' _ => True
       | Read' _ => True
       | Write' _ _ => True
-      | Seq' p1 p2 => vc pre p1
+      | Seq' _ _ p1 p2 => vc pre p1
         /\ forall v, vc (spost pre p1 (Halted v)) (p2 v)
-      | If' P Q b p1 p2 => vc (pre /\ [P]) p1 /\ vc (pre /\ [Q]) p2
+      | If' _ P Q b p1 p2 => vc (pre /\ [P]) p1 /\ vc (pre /\ [Q]) p2
       | For' nocrash crashed f n =>
         (forall m, nocrash ghost m --> crashed ghost)
         /\ (pre --> nocrash ghost 0)
         /\ (forall m, m < n -> vc (nocrash ghost m) (f m))
         /\ (forall m r, m < n -> (spost (nocrash ghost m) (f m) r -->
-          ([r = Halted 0] /\ nocrash ghost (S m)) \/ ([r = Crashed] /\ crashed ghost)))
-      | Call' cpre cp cpost c => pre --> (cpre ghost)
+          ([r = Halted tt] /\ nocrash ghost (S m)) \/ ([r = Crashed] /\ crashed ghost)))
+      | Call' _ cpre cp cpost c => pre --> (cpre ghost)
     end.
 
-  Lemma spost_sound' : forall p pre,
-    vc pre p
+  Lemma spost_sound' : forall R p pre,
+    @vc R pre p
     -> corr pre (prog'Out p) (spost pre p).
   Proof.
     induction p; simpl; intuition.
@@ -308,8 +314,8 @@ Section prog'.
     - eauto.
   Qed.
 
-  Theorem spost_sound : forall p pre post,
-    vc pre p
+  Theorem spost_sound : forall R p pre post,
+    @vc R pre p
     -> (forall r, spost pre p r --> post r)
     -> corr pre (prog'Out p) post.
   Proof.
@@ -317,18 +323,18 @@ Section prog'.
   Qed.
 End prog'.
 
-Implicit Arguments Halt' [ghostT].
-Implicit Arguments Crash' [ghostT].
+Implicit Arguments Halt' [ghostT R].
+Implicit Arguments Crash' [ghostT R].
 Implicit Arguments Read' [ghostT].
 Implicit Arguments Write' [ghostT].
-Implicit Arguments Call' [ghostT pre p post].
+Implicit Arguments Call' [ghostT R pre p post].
 
 Notation "'Halt'" := Halt' : prog'_scope.
 Notation "'Crash'" := Crash' : prog'_scope.
 Notation "!" := Read' : prog'_scope.
 Infix "<--" := Write' : prog'_scope.
 Notation "'Call'" := Call' : prog'_scope.
-Notation "p1 ;; p2" := (Seq' p1 (fun _ => p2)) : prog'_scope.
+Notation "p1 ;; p2" := (Seq' p1 (fun _ : unit => p2)) : prog'_scope.
 Notation "x <- p1 ; p2" := (Seq' p1 (fun x => p2)) : prog'_scope.
 Delimit Scope prog'_scope with prog'.
 Bind Scope prog'_scope with prog'.
@@ -340,7 +346,7 @@ Notation "'For' i < n 'Ghost' g 'Invariant' nocrash 'OnCrash' crashed 'Begin' bo
 Notation "'If' b { p1 } 'else' { p2 }" := (If' b p1 p2) (at level 9, b at level 0)
   : prog'_scope.
 
-Notation "$( ghostT : p )" := (prog'Out (p%prog' : prog' ghostT))
+Notation "$( ghostT : p )" := (prog'Out (p%prog' : prog' ghostT _))
   (ghostT at level 0).
 
 
@@ -442,13 +448,13 @@ Inductive logstate :=
 
 Module Type LOG.
   (* Methods *)
-  Parameter init : xparams -> prog.
-  Parameter begin : xparams -> prog.
-  Parameter commit : xparams -> prog.
-  Parameter abort : xparams -> prog.
-  Parameter recover : xparams -> prog.
-  Parameter read : xparams -> addr -> prog.
-  Parameter write : xparams -> addr -> valu -> prog.
+  Parameter init : xparams -> prog unit.
+  Parameter begin : xparams -> prog unit.
+  Parameter commit : xparams -> prog unit.
+  Parameter abort : xparams -> prog unit.
+  Parameter recover : xparams -> prog unit.
+  Parameter read : xparams -> addr -> prog valu.
+  Parameter write : xparams -> addr -> valu -> prog unit.
 
   (* Representation invariant *)
   Parameter rep : xparams -> logstate -> pred.
@@ -754,7 +760,7 @@ Module Log : LOG.
     If (eq_nat_dec com 1) {
       (Call (apply_ok xp))
     } else {
-      Halt 0
+      Halt tt
     }
   ).
 
@@ -794,7 +800,7 @@ Module Log : LOG.
         v <- !(LogStart xp + i*2 + 1);
         (Temp xp) <-- v
       } else {
-        Halt 0
+        Halt tt
       }
     Pool;;
 
